



$$1) y = \beta_1 x_1 + \dots + \beta_p x_p + \varepsilon$$

$$\hat{\beta}_\lambda^R = (x^T x + \lambda I_n)^{-1} x^T y$$

$$E[\hat{\beta}_\lambda^R] = E[(x^T x + \lambda I)^{-1} x^T y]$$

$$= (x^T x + \lambda I)^{-1} x^T \cdot E\{y\}$$

$$= (x^T x + \lambda I)^{-1} x^T \cdot x \beta$$

$$E[\hat{\beta}_\lambda^R] - \beta = (x^T x + \lambda I)^{-1} x^T x \beta - \beta$$

$$= [(x^T x + \lambda I)^{-1} x^T x - I] \beta$$

$$= [(x^T x + \lambda I)^{-1} (x^T x + \lambda I - \lambda I) - I] \beta$$

$$= [I - \lambda (x^T x + \lambda I)^{-1} - I] \beta$$

$$= -\lambda \underline{(x^T x + \lambda I)^{-1}} \beta$$

$$2) \quad \pi(x_1, \dots, x_p) = \frac{1}{1 + e^{-(\beta_0 + \beta_1 x_1 + \dots + \beta_p x_p)}} = \frac{1}{1 + e^{-z}}, \text{ where } z = \beta_0 + \beta^T x$$

$$\text{to show: } \nabla \pi = \pi(1-\pi)\beta$$

$$\beta^T = (\beta_1, \dots, \beta_p)$$

$$\frac{d\pi}{dz} = \pi(1-\pi)$$

$$\frac{\partial z}{\partial x_i} = \frac{\partial \pi}{\partial z} \cdot \frac{\partial z}{\partial x_i} = \pi(1-\pi)\beta_i$$

$$\therefore \nabla \pi = \begin{bmatrix} \frac{\partial \pi}{\partial x_1} \\ \vdots \\ \frac{\partial \pi}{\partial x_n} \end{bmatrix} = \pi(1-\pi) \begin{bmatrix} \beta_1 \\ \beta_2 \\ \vdots \\ \beta_p \end{bmatrix} = \pi(1-\pi)\beta$$

$$3) E[y] = a + bx = \lambda_i \quad \text{Var}[y_i] = \lambda_i$$

$$f(y) = \frac{e^{-(a+bx)} (a+bx)^y}{y!}$$

$$\text{log likelihood: } \sum_{i=1}^n \left[ -(a+bx_i) + y_i \cdot \log(a+bx_i) - \log(y_i!) \right]$$

→ 0

$$\frac{\partial \ell}{\partial a} = \sum_{i=1}^n \left[ -1 + \frac{y_i}{a+bx_i} \right] = 0$$

$$\therefore \sum \frac{y_i}{a+bx_i} = n$$

$$\frac{1}{n} \cdot \frac{\sum y_i}{\hat{a} + \hat{b}x_i} = 1$$

$$\frac{\partial \ell}{\partial b} = \sum_{i=1}^n \left[ -x_i + \frac{x_i y_i}{a+bx_i} \right]$$

$$= \sum_{i=1}^n \frac{x_i y_i}{a+bx_i} = \sum_{i=1}^n x_i$$

$$\frac{1}{n} \cdot \sum_{i=1}^n \left[ \frac{x_i y_i}{\hat{a} + \hat{b}x_i} \right] = \frac{\sum x_i}{n} = \bar{x}$$

with  $a=0$

$$\ell(b) = \sum_{i=1}^n \left[ -bx_i + y_i \cdot \log(bx_i) \right]$$

$$\frac{\partial \ell}{\partial b} = \sum -x_i + \frac{y_i}{b} = 0$$

$$\hat{b} = \frac{\sum y_i}{\sum x_i}$$

$$\text{Var}[\hat{b}], \text{ let } S_y = \sum y_i$$

$$\text{since } y_i \sim \text{Poisson}(bx_i).$$

$$S_y \sim \text{Poisson}(b \sum x_i)$$

$$\hat{b} = \frac{S_y}{\sum x_i}$$

$$E[\hat{b}] = b.$$

$$\begin{aligned} \text{Var}[\hat{b}] &= \frac{1}{(\sum x_i)^2} \cdot \text{Var}(S_y) = \frac{1}{(\sum x_i)^2} \cdot b(\sum x_i) \\ &= \frac{b}{\sum x_i} \end{aligned}$$

# HW6 Q1

$$y = \beta_1 x_1 + \dots + \beta_p x_p + \varepsilon$$

$$\hat{\beta}_\lambda^R = (X^T X + \lambda I)^{-1} X^T y$$

$$E[\hat{\beta}_\lambda^R] = E[(X^T X + \lambda I)^{-1} X^T y]$$

$$E[\hat{\beta}_\lambda^R] = -\lambda (X^T X + \lambda I_n)^{-1} \beta + \beta$$

$$= (X^T X + \lambda I_n)^{-1} X^T X \beta - \beta$$

$$= (X^T X + \lambda I_n)^{-1} X^T X \beta - (X^T X + \lambda I_n)^{-1} (X^T X + \lambda I_n) \beta$$

$$= (X^T X + \lambda I_n)^{-1} \beta [X^T X - (X^T X + \lambda I_n)]$$

$$= (X^T X + \lambda I_n)^{-1} \beta [-\lambda I_n]$$

$$= -\lambda (X^T X + \lambda I_n)^{-1} \beta$$

2)

$$\pi(x_1, \dots, x_p) = \frac{1}{1 + e^{-z}} \beta = \frac{1}{1 + e^{-z}}$$

$$\nabla \pi = \pi(1-\pi) \beta.$$

$$\frac{d\pi}{dz} = \frac{(1 + e^{-z}) \cdot 0 - (1)(0 + e^{-z} \cdot -1)}{(1 + e^{-z})^2}$$

$$= \frac{e^{-z}}{(1 + e^{-z})^2} = \frac{1}{1 + e^{-z}} \cdot \frac{e^{-z}}{1 + e^{-z}}$$

$$= \pi(1-\pi)$$

$$\frac{d\pi}{dx} = \frac{d\pi}{dz} \cdot \frac{dz}{dx} = \pi(1-\pi) \cdot \beta$$

### HW6 Q3

$$L = \prod_{i=1}^n \frac{e^{-a-bx_i} (a+bx_i)^{y_i}}{y_i!}$$

$$\ell = \log \left[ \prod_{i=1}^n \frac{e^{-a-bx_i} (a+bx_i)^{y_i}}{y_i!} \right]$$

$\ell/p - N$   
 $O.P / G.L.L - t.dist$

$$\begin{aligned} &= \sum_{i=1}^n \log (e^{-a-bx_i}) + \log (a+bx_i)^{y_i} \\ &\quad - \log (y_i!) \\ &= \sum_{i=1}^n -a - bx_i + y_i \log (a+bx_i) \\ &\quad - \log (y_i!) \end{aligned}$$

$$\hat{a} = \frac{\partial \ell}{\partial a} = \sum -1 + y_i \frac{1}{a+bx_i} \cdot (1+0) = 0$$

$$= \sum 1 + \frac{y_i}{a+bx_i}$$

$$0 = -n + \sum \frac{y_i}{a+bx_i}$$

$$1 = \frac{1}{n} \sum \frac{y_i}{a+bx_i}$$



$$\frac{\partial \ell}{\partial b} = \sum_{i=1}^n (-a - bx_i) + y_i \log(a + bx_i) - \log(y_i!)$$

$$= -x_i + \frac{y_i}{a + bx_i} \cdot x_i - 0$$

$$= -x_i + \frac{x_i y_i}{a + bx_i} = \sum x = \sum \frac{x_i y_i}{a + bx_i}$$

$$= \bar{x} = \frac{1}{n} \frac{\sum x_i y_i}{a + bx_i}$$